Auto/Translation/LamReif.lean
@@ -665,6 +665,33 @@ section Checker
 
   -- Functions that turns data structure in `ReifM.State` into `Expr`
 
+end Checker
+
+
+section BuildChecker
+
+  inductive BuildMode where
+    | small_step
+    | small_step_reflection
+  deriving BEq, Hashable, Inhabited
+
+  instance : ToString BuildMode where
+    toString : BuildMode → String
+    | .small_step => "small_step"
+    | .small_step_reflection => "small_step_reflection"
+  
+  instance : Lean.KVMap.Value BuildMode where
+    toDataValue n := toString n
+    ofDataValue?
+    | "small_step" => some .small_step
+    | "small_step_reflection" => some .small_step_reflection
+    | _ => none
+
+  register_option auto.checker.buildMode : BuildMode := {
+    defValue := BuildMode.small_step
+    descr := "Mode when building the checker"
+  }
+
   def buildChkStepsExpr : ReifM Expr := do
     let chkMap ← getChkMap
     let mut chkSteps := #[]
@@ -759,7 +786,7 @@ section Checker
 
   -- `re` is the entry we want to retrieve from the `validTable`
   -- The `expr` returned is a proof of the `LamThmValid`-ness of the entry
-  def buildFullCheckerExprFor (re : REntry) : ReifM Expr := do
+  def buildFullCheckerExprFor_smallStep (re : REntry) : ReifM Expr := do
     printCheckerStats
     let startTime ← IO.monoMsNow
     let u ← getU
@@ -790,7 +817,60 @@ section Checker
       return getEntry
     return checker
 
-end Checker
+  private def mkNativeAuxDecl (baseName : Name) (type value : Expr) : MetaM Name := do
+    -- TODO: Fix
+    let auxName := baseName ++ (.str .anonymous (toString (← getEnv).constants.size))
+    let decl := Declaration.defnDecl {
+      name := auxName, levelParams := [], type, value
+      hints := .abbrev
+      safety := .safe
+    }
+    addDecl decl
+    compileDecl decl
+    return auxName
+
+  def buildFullCheckerExprFor_smallStep_reflection (re : REntry) : ReifM Expr := do
+    printCheckerStats
+    let startTime ← IO.monoMsNow
+    let u ← getU
+    let lvtExpr := Lean.toExpr (BinTree.ofListGet ((← getVarVal).map Prod.snd).data)
+    let litExpr := Lean.toExpr (BinTree.ofListGet (← getLamILTy).data)
+    let cpvExpr ← buildCPValExpr
+    let cpvTy := Expr.const ``CPVal [u]
+    let checker ← Meta.withLetDecl `cpval cpvTy cpvExpr fun cpvFVarExpr => do
+      let (itExpr, ifExpr) ← buildImportTableExpr cpvFVarExpr
+      let csExpr ← buildChkStepsExpr
+      let .some (lctx, t) := re.getValid?
+        | throwError "buildFullCheckerExprFor :: {re} is not a `valid` entry"
+      let vExpr := Lean.toExpr (← lookupREntryPos! re)
+      let hImportExpr ← Meta.mkAppM ``Eq.refl #[ifExpr]
+      let hLvtExpr ← Meta.mkAppM ``Eq.refl #[lvtExpr]
+      let hLitExpr ← Meta.mkAppM ``Eq.refl #[litExpr]
+      let runResultExpr := Lean.mkApp3 (.const ``RTable.mk [])
+        (Lean.toExpr (← getRTableTree)) (Lean.toExpr (← getMaxEVarSucc))
+        (Lean.toExpr (← getLamEVarTyTree))
+      let runEqBoolExpr := Lean.mkApp5 (.const ``Checker.getValidExport_smallStep_reflection_runEq [])
+        lvtExpr litExpr ifExpr csExpr runResultExpr
+      let runEqNativeName ← mkNativeAuxDecl "lam_small_refl" (Lean.mkConst ``Bool) runEqBoolExpr
+      let runEqRflPrf ← Meta.mkEqRefl (toExpr true)
+      let runEqExpr := mkApp3 (Lean.mkConst ``Lean.ofReduceBool) (Lean.mkConst runEqNativeName) (toExpr true) runEqRflPrf
+      let heqExpr ← Meta.mkAppM ``Eq.refl #[← Meta.mkAppM ``Option.some #[Lean.toExpr (lctx, t)]]
+      let getEntry := Lean.mkAppN (.const ``Checker.getValidExport_smallStep_reflection [u])
+        #[cpvExpr, itExpr, csExpr, vExpr, ifExpr, hImportExpr,
+          lvtExpr, litExpr, hLvtExpr, hLitExpr, runResultExpr, runEqExpr,
+          Lean.toExpr lctx, Lean.toExpr t, heqExpr]
+      let getEntry ← Meta.mkLetFVars #[cpvFVarExpr] getEntry
+      trace[auto.buildChecker] "Checker expression built in time {(← IO.monoMsNow) - startTime}ms"
+      return getEntry
+    return checker
+
+  def buildFullCheckerExprFor (re : REntry) : ReifM Expr := do
+    let buildMode := auto.checker.buildMode.get (← getOptions)
+    match buildMode with
+    | .small_step => buildFullCheckerExprFor_smallStep re
+    | .small_step_reflection => buildFullCheckerExprFor_smallStep_reflection re
+
+end BuildChecker
 
 -- This section should only be used when exporting terms to external provers
 section ExportUtils
